\documentclass{article}
\title{Linear algebra homework rework 2025/09/29}
\author{largeoyos}
\date{\today}
\usepackage{amsmath}
\usepackage{setspace}


\begin{document}
\maketitle{Problem.4}


$$\left|
\begin{matrix}
x_{1}&y &\cdots&y \\ z&x_{2}&\cdots&y \\ \vdots&\vdots&\ddots&\vdots \\ z&z&\cdots&x_{n}
\end{matrix}
\right|=\begin{vmatrix}
x_{1}&y&\cdots&y \\ z&x_2&\cdots&y \\ \vdots&\vdots&\ddots&\vdots& \\ z&z&\cdots&y+(x_{n}-y)
\end{vmatrix}=(x_{n}-y)\cdot D_{n-1}+\begin{vmatrix}
x_{1}&y&y&\cdots&y&y \\ z&x_{2}&y&\cdots&y&y \\ z&z&x_{3}&\cdots &y &y \\ \vdots&\vdots&\vdots&\ddots&\vdots&\vdots \\ z&z&z&\cdots&x_{n-1}&y \\ z&z&z&\cdots&z&y
\end{vmatrix}$$

$$=(x_{n}-y)\cdot D_{n-1}+\begin{vmatrix}
x_{1}&y &y &\cdots&y&y \\ z-x_{1}&x_2-y&0&\cdots&0&0 \\ z-x_{1}&z-y&0 &\cdots&0&0 \\ \vdots & \vdots & \vdots & \ddots & \vdots & \vdots \\ z-x_{1} & z-y & z-y & \cdots & x_{n-1}-y  & 0 \\ z-x_{1} & z-y & z-y & \cdots & z-y & 0 \\ 
\end{vmatrix}_{n}$$
$$=(x_{n}-y)\cdot D_{n-1}+(-1)^{n+1}y\begin{vmatrix}
z-x_{1} & x_{2}-y & 0 & \cdots & 0  &  \\ z-x_{1} & z-y & x_{3}-y & \cdots &0 \\ \vdots & \vdots & \vdots & \ddots & \vdots \\ z-x_{1} & z-y  & z-y & \cdots & x_{n-1}-y \\ z-x_{1} & z-y & z-y & \cdots &  z-y 
\end{vmatrix}_{n-1}$$
$$=(x_{n}-y)\cdot D_{n-1}+(-1)^{n+1}y\begin{vmatrix}
z-x_{1} & x_{2}-y & 0 & \cdots & 0  &  \\ 0 & z-x_{2} & x_{3}-y & \cdots &0 \\ \vdots & \vdots & \vdots & \ddots & \vdots \\ 0 & 0  & 0 & \cdots & x_{n-1}-y \\ 0 & 0 & 0 & \cdots &  z-x_{n-1} 
\end{vmatrix}_{n-1}$$
$$=(x_{n}-y)\cdot D_{n-1}+(-1)^{n+1}y\cdot \prod_{i=1}^{n-1}(z-x_{i})$$
    Hence $D_{n}=(x_{n}-y)\cdot+y\cdot\prod^{n-1}_{i=1}(x_{i}-z)$ \\
    Similarly, $D_{n}=(x_{n}-z)\cdot+y\cdot\prod^{n-1}_{i=1}(x_{i}-y)$ \\
   
    \large {when $y\neq z$ , $D_{n}=\frac{y\prod^{n}_{i=1}(x_{i}-z)-x\prod^{n}_{i=1}(x_{i}-y)}{y-z}$}

 



\end{document}
